Progress.

smc/SMC.ec
@@ -677,6 +677,8 @@ module SMCSim (Adv : FUNC) = {
 
 (* simplified version of SMCReal(KeyEx.KEIdeal) *)
 
+abstract theory SMCRealKEIdealSimp.
+
 type smc_real_ke_ideal_simp_state = [
     SMCRealKEIdealSimpStateWaitReq
   | SMCRealKEIdealSimpStateWaitAdv1 of (port * port * bits)
@@ -840,7 +842,7 @@ module SMCRealKEIdealSimp : FUNC = {
         (addr1, addr2) <- oget (Fwd.dec_fw_ok m);
         if (addr1 = self ++ [1]) {
           (* destination of m is (self ++ [1], 1), mode of m is Adv *)
-          r <- Some (smc_rsp self pt1 pt2 (x ^^ k));
+          r <- Some (smc_rsp self pt1 pt2 x);
           st <- SMCRealKEIdealSimpStateFinal (pt1, pt2, x, k);
         }
       }
@@ -860,6 +862,230 @@ module SMCRealKEIdealSimp : FUNC = {
     return r;
   }
 }.
+
+(* relational invariant for connecting SMCReal(KeyEx.KEIdeal) and
+   SMCRealKEIdealSimp *)
+
+type smc_real_ke_ideal_simp_rel_st = {
+  smc_real_ke_ideal_simp_rel_st_func : addr;
+  smc_real_ke_ideal_simp_rel_st_r1s  : smc_real_p1_state;
+  smc_real_ke_ideal_simp_rel_st_r2s  : smc_real_p2_state;
+  smc_real_ke_ideal_simp_rel_st_fws  : Fwd.fw_state;
+  smc_real_ke_ideal_simp_rel_st_keis : KeyEx.ke_ideal_state;
+  smc_real_ke_ideal_simp_rel_st_riss : smc_real_ke_ideal_simp_state;
+}.
+
+pred smc_real_ke_ideal_simp_rel0 (st : smc_real_ke_ideal_simp_rel_st) =
+  (st.`smc_real_ke_ideal_simp_rel_st_r1s  = SMCRealP1StateWaitReq) /\
+  (st.`smc_real_ke_ideal_simp_rel_st_r2s  = SMCRealP2StateWaitKE1) /\
+  (st.`smc_real_ke_ideal_simp_rel_st_fws  = Fwd.FwStateInit) /\
+  (st.`smc_real_ke_ideal_simp_rel_st_keis = KeyEx.KEIdealStateWaitReq1) /\
+  (st.`smc_real_ke_ideal_simp_rel_st_riss = SMCRealKEIdealSimpStateWaitReq).
+
+pred smc_real_ke_ideal_simp_rel1
+     (st : smc_real_ke_ideal_simp_rel_st, pt1 pt2 : port, x : bits) =
+  ! (st.`smc_real_ke_ideal_simp_rel_st_func <= pt1.`1) /\
+  ! (st.`smc_real_ke_ideal_simp_rel_st_func <= pt2.`1) /\
+  (st.`smc_real_ke_ideal_simp_rel_st_r1s  =
+   SMCRealP1StateWaitKE2 (pt1, pt2, x)) /\
+  (st.`smc_real_ke_ideal_simp_rel_st_r2s  = SMCRealP2StateWaitKE1) /\
+  (st.`smc_real_ke_ideal_simp_rel_st_fws  = Fwd.FwStateInit) /\
+  (st.`smc_real_ke_ideal_simp_rel_st_keis =
+   KeyEx.KEIdealStateWaitSim1
+   ((st.`smc_real_ke_ideal_simp_rel_st_func, 3),
+    (st.`smc_real_ke_ideal_simp_rel_st_func, 4))) /\
+  (st.`smc_real_ke_ideal_simp_rel_st_riss =
+   SMCRealKEIdealSimpStateWaitAdv1 (pt1, pt2, x)).
+
+pred smc_real_ke_ideal_simp_rel2
+     (st : smc_real_ke_ideal_simp_rel_st, pt1 pt2 : port,
+      x : bits, q : exp) =
+  ! (st.`smc_real_ke_ideal_simp_rel_st_func <= pt1.`1) /\
+  ! (st.`smc_real_ke_ideal_simp_rel_st_func <= pt2.`1) /\
+  (st.`smc_real_ke_ideal_simp_rel_st_r1s  =
+   SMCRealP1StateWaitKE2 (pt1, pt2, x)) /\
+  (st.`smc_real_ke_ideal_simp_rel_st_r2s  =
+   SMCRealP2StateWaitFwd (g ^ q)) /\
+  (st.`smc_real_ke_ideal_simp_rel_st_fws  = Fwd.FwStateInit) /\
+  (st.`smc_real_ke_ideal_simp_rel_st_keis =
+   KeyEx.KEIdealStateWaitSim2
+   ((st.`smc_real_ke_ideal_simp_rel_st_func, 3),
+    (st.`smc_real_ke_ideal_simp_rel_st_func, 4),
+    q)) /\
+  (st.`smc_real_ke_ideal_simp_rel_st_riss =
+   SMCRealKEIdealSimpStateWaitAdv2 (pt1, pt2, x, g ^ q)).
+
+pred smc_real_ke_ideal_simp_rel3
+     (st : smc_real_ke_ideal_simp_rel_st, pt1 pt2 : port,
+      x : bits, q : exp) =
+  ! (st.`smc_real_ke_ideal_simp_rel_st_func <= pt1.`1) /\
+  ! (st.`smc_real_ke_ideal_simp_rel_st_func <= pt2.`1) /\
+  (st.`smc_real_ke_ideal_simp_rel_st_r1s  =
+   SMCRealP1StateFinal (pt1, pt2, x)) /\
+  (st.`smc_real_ke_ideal_simp_rel_st_r2s  =
+   SMCRealP2StateWaitFwd (g ^ q)) /\
+  (st.`smc_real_ke_ideal_simp_rel_st_fws  =
+   Fwd.FwStateWait
+   ((st.`smc_real_ke_ideal_simp_rel_st_func, 3),
+    (st.`smc_real_ke_ideal_simp_rel_st_func, 4),
+    univ_triple (UnivPort pt1) (UnivPort pt2)
+                (UnivBase (BaseBits (x ^^ (g ^ q)))))) /\
+  (st.`smc_real_ke_ideal_simp_rel_st_keis =
+   KeyEx.KEIdealStateFinal
+   ((st.`smc_real_ke_ideal_simp_rel_st_func, 3),
+    (st.`smc_real_ke_ideal_simp_rel_st_func, 4),
+    q)) /\
+  (st.`smc_real_ke_ideal_simp_rel_st_riss =
+   SMCRealKEIdealSimpStateWaitAdv3 (pt1, pt2, x, g ^ q)).
+
+pred smc_real_ke_ideal_simp_rel4
+     (st : smc_real_ke_ideal_simp_rel_st, pt1 pt2 : port,
+      x : bits, q : exp) =
+  ! (st.`smc_real_ke_ideal_simp_rel_st_func <= pt1.`1) /\
+  ! (st.`smc_real_ke_ideal_simp_rel_st_func <= pt2.`1) /\
+  (st.`smc_real_ke_ideal_simp_rel_st_r1s  =
+   SMCRealP1StateFinal (pt1, pt2, x)) /\
+  (st.`smc_real_ke_ideal_simp_rel_st_r2s  =
+   SMCRealP2StateFinal (g ^ q)) /\
+  (st.`smc_real_ke_ideal_simp_rel_st_fws  =
+   Fwd.FwStateFinal
+   ((st.`smc_real_ke_ideal_simp_rel_st_func, 3),
+    (st.`smc_real_ke_ideal_simp_rel_st_func, 4),
+    univ_triple (UnivPort pt1) (UnivPort pt2)
+                (UnivBase (BaseBits (x ^^ (g ^ q)))))) /\
+  (st.`smc_real_ke_ideal_simp_rel_st_keis =
+   KeyEx.KEIdealStateFinal
+   ((st.`smc_real_ke_ideal_simp_rel_st_func, 3),
+    (st.`smc_real_ke_ideal_simp_rel_st_func, 4),
+    q)) /\
+  (st.`smc_real_ke_ideal_simp_rel_st_riss =
+   SMCRealKEIdealSimpStateFinal (pt1, pt2, x, g ^ q)).
+
+inductive smc_real_ke_ideal_simp_rel
+          (st : smc_real_ke_ideal_simp_rel_st) =
+    SMCRealKEIdealSimpRel0 of (smc_real_ke_ideal_simp_rel0 st)
+  | SMCRealKEIdealSimpRel1 (pt1 pt2 : port, x : bits) of
+      (smc_real_ke_ideal_simp_rel1 st pt1 pt2 x)
+  | SMCRealKEIdealSimpRel2 (pt1 pt2 : port, x : bits, q : exp) of
+      (smc_real_ke_ideal_simp_rel2 st pt1 pt2 x q)
+  | SMCRealKEIdealSimpRel3 (pt1 pt2 : port, x : bits, q : exp) of
+      (smc_real_ke_ideal_simp_rel3 st pt1 pt2 x q)
+  | SMCRealKEIdealSimpRel4 (pt1 pt2 : port, x : bits, q : exp) of
+      (smc_real_ke_ideal_simp_rel4 st pt1 pt2 x q).
+
+lemma SMCReal_KEIdeal_SMCRealKEIdealSimp_invoke (func adv : addr) :
+  equiv
+  [SMCReal(KeyEx.KEIdeal).invoke ~ SMCRealKEIdealSimp.invoke :
+   ! func <= adv /\ ={m} /\
+   SMCReal.self{1} = func /\ SMCReal.adv{1} = adv /\
+   Fwd.Forw.self{1} = func ++ [1] /\ Fwd.Forw.adv{1} = adv /\
+   KeyEx.KEIdeal.self{1} = func ++ [2] /\ KeyEx.KEIdeal.adv{1} = adv /\
+   SMCRealKEIdealSimp.self{2} = func /\ SMCRealKEIdealSimp.adv{2} = adv /\
+   smc_real_ke_ideal_simp_rel
+   {|smc_real_ke_ideal_simp_rel_st_func = func;
+     smc_real_ke_ideal_simp_rel_st_r1s  = SMCReal.st1{1};
+     smc_real_ke_ideal_simp_rel_st_r2s  = SMCReal.st2{1};
+     smc_real_ke_ideal_simp_rel_st_fws  = Fwd.Forw.st{1};
+     smc_real_ke_ideal_simp_rel_st_keis = KeyEx.KEIdeal.st{1};
+     smc_real_ke_ideal_simp_rel_st_riss = SMCRealKEIdealSimp.st{2}|} ==>
+   ={res} /\
+   smc_real_ke_ideal_simp_rel
+   {|smc_real_ke_ideal_simp_rel_st_func = func;
+     smc_real_ke_ideal_simp_rel_st_r1s  = SMCReal.st1{1};
+     smc_real_ke_ideal_simp_rel_st_r2s  = SMCReal.st2{1};
+     smc_real_ke_ideal_simp_rel_st_fws  = Fwd.Forw.st{1};
+     smc_real_ke_ideal_simp_rel_st_keis = KeyEx.KEIdeal.st{1};
+     smc_real_ke_ideal_simp_rel_st_riss = SMCRealKEIdealSimp.st{2}|}].
+proof.
+proc.
+case
+  (smc_real_ke_ideal_simp_rel0
+   {|smc_real_ke_ideal_simp_rel_st_func = func;
+     smc_real_ke_ideal_simp_rel_st_r1s  = SMCReal.st1{1};
+     smc_real_ke_ideal_simp_rel_st_r2s  = SMCReal.st2{1};
+     smc_real_ke_ideal_simp_rel_st_fws  = Fwd.Forw.st{1};
+     smc_real_ke_ideal_simp_rel_st_keis = KeyEx.KEIdeal.st{1};
+     smc_real_ke_ideal_simp_rel_st_riss = SMCRealKEIdealSimp.st{2}|}).
+admit.
+admit.
+qed.
+
+lemma Exper_SMCReal_KEIdeal_SMCRealKEIdealSimp
+      (func' adv' : addr) (in_guard' : int fset) &m
+      (Adv <: FUNC{MI, SMCReal, KeyEx.KEIdeal, SMCRealKEIdealSimp})
+      (Env <: ENV{MI, SMCReal, KeyEx.KEIdeal, SMCRealKEIdealSimp, Adv}) :
+  ! func' <= adv' =>
+  Pr[Exper(MI(SMCReal(KeyEx.KEIdeal), Adv), Env).main
+       (func', adv', in_guard') @ &m : res] =
+  Pr[Exper(MI(SMCRealKEIdealSimp, Adv), Env).main
+       (func', adv', in_guard') @ &m : res].
+proof.
+move => pre.
+byequiv => //; proc; inline*.
+seq 23 12 :
+  (! func' <= adv' /\ ={func, adv, in_guard, glob Adv, glob MI} /\
+   func{1} = func' /\ adv{1} = adv' /\ in_guard{1} = in_guard' /\
+   MI.func{1} = func' /\ MI.adv{1} = adv' /\ MI.in_guard{1} = in_guard' /\
+   SMCReal.self{1} = func' /\ SMCReal.adv{1} = adv' /\
+   Fwd.Forw.self{1} = func' ++ [1] /\ Fwd.Forw.adv{1} = adv' /\
+   KeyEx.KEIdeal.self{1} = func' ++ [2] /\ KeyEx.KEIdeal.adv{1} = adv' /\
+   SMCRealKEIdealSimp.self{2} = func' /\ SMCRealKEIdealSimp.adv{2} = adv' /\
+   smc_real_ke_ideal_simp_rel
+   {|smc_real_ke_ideal_simp_rel_st_func = func';
+     smc_real_ke_ideal_simp_rel_st_r1s  = SMCReal.st1{1};
+     smc_real_ke_ideal_simp_rel_st_r2s  = SMCReal.st2{1};
+     smc_real_ke_ideal_simp_rel_st_fws  = Fwd.Forw.st{1};
+     smc_real_ke_ideal_simp_rel_st_keis = KeyEx.KEIdeal.st{1};
+     smc_real_ke_ideal_simp_rel_st_riss = SMCRealKEIdealSimp.st{2}|}).
+call (_ : true).
+auto; progress;
+  by rewrite SMCRealKEIdealSimpRel0 /smc_real_ke_ideal_simp_rel0.
+call
+  (_ :
+   ! func' <= adv' /\ ={glob Adv, glob MI} /\
+   MI.func{1} = func' /\ MI.adv{1} = adv' /\ MI.in_guard{1} = in_guard' /\
+   SMCReal.self{1} = func' /\ SMCReal.adv{1} = adv' /\
+   Fwd.Forw.self{1} = func' ++ [1] /\ Fwd.Forw.adv{1} = adv' /\
+   KeyEx.KEIdeal.self{1} = func' ++ [2] /\ KeyEx.KEIdeal.adv{1} = adv' /\
+   SMCRealKEIdealSimp.self{2} = func' /\ SMCRealKEIdealSimp.adv{2} = adv' /\
+   smc_real_ke_ideal_simp_rel
+   {|smc_real_ke_ideal_simp_rel_st_func = func';
+     smc_real_ke_ideal_simp_rel_st_r1s  = SMCReal.st1{1};
+     smc_real_ke_ideal_simp_rel_st_r2s  = SMCReal.st2{1};
+     smc_real_ke_ideal_simp_rel_st_fws  = Fwd.Forw.st{1};
+     smc_real_ke_ideal_simp_rel_st_keis = KeyEx.KEIdeal.st{1};
+     smc_real_ke_ideal_simp_rel_st_riss = SMCRealKEIdealSimp.st{2}|}).
+proc.
+sp 2 2.
+if => //.
+inline MI(SMCReal(KeyEx.KEIdeal), Adv).loop
+       MI(SMCRealKEIdealSimp, Adv).loop.
+wp; sp.
+while
+  (={not_done, m0, r0} /\ 
+   ! func' <= adv' /\ ={glob Adv, glob MI} /\
+   MI.func{1} = func' /\ MI.adv{1} = adv' /\ MI.in_guard{1} = in_guard' /\
+   SMCReal.self{1} = func' /\ SMCReal.adv{1} = adv' /\
+   Fwd.Forw.self{1} = func' ++ [1] /\ Fwd.Forw.adv{1} = adv' /\
+   KeyEx.KEIdeal.self{1} = func' ++ [2] /\ KeyEx.KEIdeal.adv{1} = adv' /\
+   SMCRealKEIdealSimp.self{2} = func' /\ SMCRealKEIdealSimp.adv{2} = adv' /\
+   smc_real_ke_ideal_simp_rel
+   {|smc_real_ke_ideal_simp_rel_st_func = func';
+     smc_real_ke_ideal_simp_rel_st_r1s  = SMCReal.st1{1};
+     smc_real_ke_ideal_simp_rel_st_r2s  = SMCReal.st2{1};
+     smc_real_ke_ideal_simp_rel_st_fws  = Fwd.Forw.st{1};
+     smc_real_ke_ideal_simp_rel_st_keis = KeyEx.KEIdeal.st{1};
+     smc_real_ke_ideal_simp_rel_st_riss = SMCRealKEIdealSimp.st{2}|}).
+sp 2 2.
+if => //.
+wp; call (SMCReal_KEIdeal_SMCRealKEIdealSimp_invoke func' adv'); auto.
+wp; call (_ : true); auto.
+auto.
+auto.
+auto.
+qed.
+
+end SMCRealKEIdealSimp.
 
 (* make fresh version of MI *)
 
@@ -990,11 +1216,11 @@ qed.
 end section.
 
 lemma smc_security1
-        (Adv <: FUNC{MI, SMCReal, KeyEx.KEReal, KeyEx.KEIdeal,
-                     KeyEx.KESim, KeyEx.DDH_Adv, CompEnv})
-        (Env <: ENV{Adv, MI, SMCReal, KeyEx.KEReal, KeyEx.KEIdeal,
-                    KeyEx.KESim, KeyEx.DDH_Adv, CompEnv})
-        (func adv : addr) &m :
+      (Adv <: FUNC{MI, SMCReal, KeyEx.KEReal, KeyEx.KEIdeal,
+                   KeyEx.KESim, KeyEx.DDH_Adv, CompEnv})
+      (Env <: ENV{Adv, MI, SMCReal, KeyEx.KEReal, KeyEx.KEIdeal,
+                  KeyEx.KESim, KeyEx.DDH_Adv, CompEnv})
+      (func adv : addr) &m :
   exper_pre func adv (fset1 adv_fw_pi) =>
   KeyEx.DDH_Adv.func{m} = func ++ [2] => KeyEx.DDH_Adv.adv{m} = adv =>
   `|Pr[Exper(MI(SMCReal(KeyEx.KEReal), Adv), Env).main
@@ -1016,603 +1242,12 @@ rewrite /involutive /cancel /pad_iso => q.
 by rewrite gen_logK xorA xorK xor_0 log_genK.
 qed.
 
-(*
-type smc_sec2_st = {
-  smc_sec2_st_func  : addr;
-  smc_sec2_st_smcrs : smc_real_state;
-  smc_sec2_st_fws   : Fwd.fw_state;
-  smc_sec2_st_keis  : KeyEx.ke_ideal_state;
-  smc_sec2_st_smcis : smc_ideal_state;
-  smc_sec2_st_smcss : smc_sim_state
-}.
-
-pred smc_sec2_rel0 (st : smc_sec2_st) =
-  (st.`smc_sec2_st_smcrs = SMCRealStateWaitReq) /\
-  (st.`smc_sec2_st_fws   = Fwd.FwStateInit) /\
-  (st.`smc_sec2_st_keis  = KeyEx.KEIdealStateWaitReq1) /\
-  (st.`smc_sec2_st_smcis = SMCIdealStateWaitReq) /\
-  (st.`smc_sec2_st_smcss = SMCSimStateWaitReq).
-
-pred smc_sec2_rel1 (st : smc_sec2_st, pt1 pt2 : port, x : bits, q : exp) =
-  ! st.`smc_sec2_st_func <= pt1.`1 /\ ! st.`smc_sec2_st_func <= pt2.`1 /\ 
-  (st.`smc_sec2_st_smcrs = SMCRealStateWaitKE1 (pt1, pt2, x)) /\
-  (st.`smc_sec2_st_fws   = Fwd.FwStateInit) /\
-  (st.`smc_sec2_st_keis  = KeyEx.KEIdealStateWaitSim1 ((st.`smc_sec2_st_func, 1), (st.`smc_sec2_st_func, 2), q)) /\
-  (st.`smc_sec2_st_smcis = SMCIdealStateWaitSim (pt1, pt2, x)) /\
-  (st.`smc_sec2_st_smcss = SMCSimStateWaitAdv1 (st.`smc_sec2_st_func, pad_iso x q)).
-
-pred smc_sec2_rel2 (st : smc_sec2_st, pt1 pt2 : port, x : bits, q : exp) =
-  ! st.`smc_sec2_st_func <= pt1.`1 /\ ! st.`smc_sec2_st_func <= pt2.`1 /\ 
-  (st.`smc_sec2_st_smcrs = SMCRealStateWaitKE2 (pt1, pt2, x, g ^ q)) /\
-  (st.`smc_sec2_st_fws   = Fwd.FwStateInit) /\
-  (st.`smc_sec2_st_keis  = KeyEx.KEIdealStateWaitSim2 ((st.`smc_sec2_st_func, 1), (st.`smc_sec2_st_func, 2), q)) /\
-  (st.`smc_sec2_st_smcis = SMCIdealStateWaitSim (pt1, pt2, x)) /\
-  (st.`smc_sec2_st_smcss = SMCSimStateWaitAdv2 (st.`smc_sec2_st_func, pad_iso x q)).
-
-pred smc_sec2_rel3 (st : smc_sec2_st, pt1 pt2 : port, x : bits, q : exp) =
-  ! st.`smc_sec2_st_func <= pt1.`1 /\ ! st.`smc_sec2_st_func <= pt2.`1 /\ 
-  (st.`smc_sec2_st_smcrs =
-     SMCRealStateWaitFwd (pt1, pt2, x, g ^ q, g ^ q)) /\
-  (st.`smc_sec2_st_fws   =
-     Fwd.FwStateWait
-     ((st.`smc_sec2_st_func, 1), (st.`smc_sec2_st_func, 2), UnivBase (BaseBits (x ^^ g ^ q)))) /\
-  (st.`smc_sec2_st_keis  = KeyEx.KEIdealStateFinal ((st.`smc_sec2_st_func, 1), (st.`smc_sec2_st_func, 2), q)) /\
-  (st.`smc_sec2_st_smcis = SMCIdealStateWaitSim (pt1, pt2, x)) /\
-  (st.`smc_sec2_st_smcss = SMCSimStateWaitAdv3 (st.`smc_sec2_st_func, pad_iso x q)).
-
-pred smc_sec2_rel4 (st : smc_sec2_st, pt1, pt2 : port, x : bits, q : exp) =
-  (st.`smc_sec2_st_smcrs = SMCRealStateFinal (pt1, pt2, x, g ^ q, g ^ q)) /\
-  (st.`smc_sec2_st_fws   =
-     Fwd.FwStateFinal
-     ((st.`smc_sec2_st_func, 1), (st.`smc_sec2_st_func, 2), UnivBase (BaseBits (x ^^ g ^ q)))) /\
-  (st.`smc_sec2_st_keis  = KeyEx.KEIdealStateFinal ((st.`smc_sec2_st_func, 1), (st.`smc_sec2_st_func, 2), q)) /\
-  (st.`smc_sec2_st_smcis = SMCIdealStateFinal (pt1, pt2, x)) /\
-  (st.`smc_sec2_st_smcss = SMCSimStateFinal (st.`smc_sec2_st_func, pad_iso x q)).
-
-inductive smc_sec2_rel (st : smc_sec2_st) =
-    SMCSec2Rel0 of (smc_sec2_rel0 st)
-  | SMCSec2Rel1 (pt1 pt2 : port, x : bits, q : exp) of
-      (smc_sec2_rel1 st pt1 pt2 x q)
-  | SMCSec2Rel2 (pt1 pt2 : port, x : bits, q : exp) of
-      (smc_sec2_rel2 st pt1 pt2 x q)
-  | SMCSec2Rel3 (pt1 pt2 : port, x : bits, q : exp) of
-      (smc_sec2_rel3 st pt1 pt2 x q)
-  | SMCSec2Rel4 (pt1 pt2 : port, x : bits, q : exp) of
-      (smc_sec2_rel4 st pt1 pt2 x q).
-
-inductive smc_sec2_rel_1_4 (st : smc_sec2_st) =
-    SMCSec2Rel1_1_4 (pt1 pt2 : port, x : bits, q : exp) of
-      (smc_sec2_rel1 st pt1 pt2 x q)
-  | SMCSec2Rel2_1_4 (pt1 pt2 : port, x : bits, q : exp) of
-      (smc_sec2_rel2 st pt1 pt2 x q)
-  | SMCSec2Rel3_1_4 (pt1 pt2 : port, x : bits, q : exp) of
-      (smc_sec2_rel3 st pt1 pt2 x q)
-  | SMCSec2Rel4_1_4 (pt1 pt2 : port, x : bits, q : exp) of
-      (smc_sec2_rel4 st pt1 pt2 x q).
-
-inductive smc_sec2_rel_2_4 (st : smc_sec2_st) =
-    SMCSec2Rel2_2_4 (pt1 pt2 : port, x : bits, q : exp) of
-      (smc_sec2_rel2 st pt1 pt2 x q)
-  | SMCSec2Rel3_2_4 (pt1 pt2 : port, x : bits, q : exp) of
-      (smc_sec2_rel3 st pt1 pt2 x q)
-  | SMCSec2Rel4_2_4 (pt1 pt2 : port, x : bits, q : exp) of
-      (smc_sec2_rel4 st pt1 pt2 x q).
-
-inductive smc_sec2_rel_3_4 (st : smc_sec2_st) =
-    SMCSec2Rel3_3_4 (pt1 pt2 : port, x : bits, q : exp) of
-      (smc_sec2_rel3 st pt1 pt2 x q)
-  | SMCSec2Rel4_3_4 (pt1 pt2 : port, x : bits, q : exp) of
-      (smc_sec2_rel4 st pt1 pt2 x q).
-
-inductive smc_sec2_rel_4_4 (st : smc_sec2_st) =
-    SMCSec2Rel4_4_4 (pt1 pt2 : port, x : bits, q : exp) of
-      (smc_sec2_rel4 st pt1 pt2 x q).
-
-lemma smc_sec2_rel_1_4_imp_full (st : smc_sec2_st) :
-  smc_sec2_rel_1_4 st => smc_sec2_rel st.
-proof.
-case;
-  [apply SMCSec2Rel1 | apply SMCSec2Rel2 | apply SMCSec2Rel3 |
-   apply SMCSec2Rel4].
-qed.
-
-lemma smc_sec2_rel_2_4_imp_full (st : smc_sec2_st) :
-  smc_sec2_rel_2_4 st => smc_sec2_rel st.
-proof.
-case; [apply SMCSec2Rel2 | apply SMCSec2Rel3 | apply SMCSec2Rel4].
-qed.
-
-lemma smc_sec2_rel_3_4_imp_full (st : smc_sec2_st) :
-  smc_sec2_rel_3_4 st => smc_sec2_rel st.
-proof.
-case; [apply SMCSec2Rel3 | apply SMCSec2Rel4].
-qed.
-
-lemma smc_sec2_rel_4_imp_full (st : smc_sec2_st) :
-  smc_sec2_rel_4_4 st => smc_sec2_rel st.
-proof.
-case; apply SMCSec2Rel4.
-qed.
-
 section.
 
-declare module Adv : FUNC{MI, SMCReal, KeyEx.KEIdeal, SMCIdeal, SMCSim}.
-declare module Env : ENV{Adv, MI, SMCReal, KeyEx.KEIdeal, SMCIdeal, SMCSim}.
+declare module Adv : FUNC{MI, SMCReal, SMCIdeal, SMCSim, KeyEx.KEIdeal}.
+declare module Env : ENV{Adv, MI, SMCReal, SMCIdeal, SMCSim, KeyEx.KEIdeal}.
 
-lemma MI_SMCReal_KEIdeal_Adv_SMCIdeal_SMCSim_Adv_invoke_4 :
-  equiv
-  [MI(SMCReal(KeyEx.KEIdeal), Adv).invoke ~
-   MI(SMCIdeal, SMCSim(Adv)).invoke :
-   ={m, MI.func, MI.adv, MI.in_guard} /\
-   exper_pre MI.func{1} MI.adv{1} (fset1 adv_fw_pi) /\
-   MI.in_guard{1} = fset1 adv_fw_pi /\
-   SMCReal.self{1} = MI.func{1} /\ SMCReal.adv{1} = MI.adv{1} /\
-   Fwd.Forw.self{1} = MI.func{1} ++ [1] /\
-   Fwd.Forw.adv{1} = MI.adv{1} /\
-   KeyEx.KEIdeal.self{1} = MI.func{1} ++ [2] /\
-   KeyEx.KEIdeal.adv{1} = MI.adv{1} /\
-   SMCIdeal.self{2} = MI.func{1} /\ SMCIdeal.adv{2} = MI.adv{1} /\
-   SMCSim.self{2} = MI.adv{1} /\ SMCSim.adv{2} = [] /\
-   ={glob Adv} /\
-   (exists (pt1 pt2 : port, x : bits, q : exp),
-    smc_sec2_rel4
-    {|smc_sec2_st_func = MI.func{1}; smc_sec2_st_smcrs = SMCReal.st{1};
-      smc_sec2_st_fws = Fwd.Forw.st{1}; smc_sec2_st_keis = KeyEx.KEIdeal.st{1};
-      smc_sec2_st_smcis = SMCIdeal.st{2}; smc_sec2_st_smcss = SMCSim.st{2}|}
-    pt1 pt2 x q) ==>
-   ={res, MI.func, MI.adv, MI.in_guard} /\
-   exper_pre MI.func{1} MI.adv{1} (fset1 adv_fw_pi) /\
-   MI.in_guard{1} = fset1 adv_fw_pi /\
-   SMCReal.self{1} = MI.func{1} /\ SMCReal.adv{1} = MI.adv{1} /\
-   Fwd.Forw.self{1} = MI.func{1} ++ [1] /\
-   Fwd.Forw.adv{1} = MI.adv{1} /\
-   KeyEx.KEIdeal.self{1} = MI.func{1} ++ [2] /\
-   KeyEx.KEIdeal.adv{1} = MI.adv{1} /\
-   SMCIdeal.self{2} = MI.func{1} /\ SMCIdeal.adv{2} = MI.adv{1} /\
-   SMCSim.self{2} = MI.adv{1} /\ SMCSim.adv{2} = [] /\
-   ={glob Adv} /\
-   smc_sec2_rel_4_4
-   {|smc_sec2_st_func = MI.func{1}; smc_sec2_st_smcrs = SMCReal.st{1};
-     smc_sec2_st_fws = Fwd.Forw.st{1}; smc_sec2_st_keis = KeyEx.KEIdeal.st{1};
-     smc_sec2_st_smcis = SMCIdeal.st{2}; smc_sec2_st_smcss = SMCSim.st{2}|}].
-proof.
-admit.
-qed.
-
-lemma MI_SMCReal_KEIdeal_Adv_SMCIdeal_SMCSim_Adv_invoke_3 :
-  equiv
-  [MI(SMCReal(KeyEx.KEIdeal), Adv).invoke ~
-   MI(SMCIdeal, SMCSim(Adv)).invoke :
-   ={m, MI.func, MI.adv, MI.in_guard} /\
-   exper_pre MI.func{1} MI.adv{1} (fset1 adv_fw_pi) /\
-   MI.in_guard{1} = fset1 adv_fw_pi /\
-   SMCReal.self{1} = MI.func{1} /\ SMCReal.adv{1} = MI.adv{1} /\
-   Fwd.Forw.self{1} = MI.func{1} ++ [1] /\
-   Fwd.Forw.adv{1} = MI.adv{1} /\
-   KeyEx.KEIdeal.self{1} = MI.func{1} ++ [2] /\
-   KeyEx.KEIdeal.adv{1} = MI.adv{1} /\
-   SMCIdeal.self{2} = MI.func{1} /\ SMCIdeal.adv{2} = MI.adv{1} /\
-   SMCSim.self{2} = MI.adv{1} /\ SMCSim.adv{2} = [] /\
-   ={glob Adv} /\
-   (exists (pt1 pt2 : port, x : bits, q : exp),
-    smc_sec2_rel3
-    {|smc_sec2_st_func = MI.func{1}; smc_sec2_st_smcrs = SMCReal.st{1};
-      smc_sec2_st_fws = Fwd.Forw.st{1}; smc_sec2_st_keis = KeyEx.KEIdeal.st{1};
-      smc_sec2_st_smcis = SMCIdeal.st{2}; smc_sec2_st_smcss = SMCSim.st{2}|}
-    pt1 pt2 x q) ==>
-   ={res, MI.func, MI.adv, MI.in_guard} /\
-   exper_pre MI.func{1} MI.adv{1} (fset1 adv_fw_pi) /\
-   MI.in_guard{1} = fset1 adv_fw_pi /\
-   SMCReal.self{1} = MI.func{1} /\ SMCReal.adv{1} = MI.adv{1} /\
-   Fwd.Forw.self{1} = MI.func{1} ++ [1] /\
-   Fwd.Forw.adv{1} = MI.adv{1} /\
-   KeyEx.KEIdeal.self{1} = MI.func{1} ++ [2] /\
-   KeyEx.KEIdeal.adv{1} = MI.adv{1} /\
-   SMCIdeal.self{2} = MI.func{1} /\ SMCIdeal.adv{2} = MI.adv{1} /\
-   SMCSim.self{2} = MI.adv{1} /\ SMCSim.adv{2} = [] /\
-   ={glob Adv} /\
-   smc_sec2_rel_3_4
-   {|smc_sec2_st_func = MI.func{1}; smc_sec2_st_smcrs = SMCReal.st{1};
-     smc_sec2_st_fws = Fwd.Forw.st{1}; smc_sec2_st_keis = KeyEx.KEIdeal.st{1};
-     smc_sec2_st_smcis = SMCIdeal.st{2}; smc_sec2_st_smcss = SMCSim.st{2}|}].
-proof.
-admit.
-qed.
-
-lemma MI_SMCReal_KEIdeal_Adv_SMCIdeal_SMCSim_Adv_invoke_2 :
-  equiv
-  [MI(SMCReal(KeyEx.KEIdeal), Adv).invoke ~
-   MI(SMCIdeal, SMCSim(Adv)).invoke :
-   ={m, MI.func, MI.adv, MI.in_guard} /\
-   exper_pre MI.func{1} MI.adv{1} (fset1 adv_fw_pi) /\
-   MI.in_guard{1} = fset1 adv_fw_pi /\
-   SMCReal.self{1} = MI.func{1} /\ SMCReal.adv{1} = MI.adv{1} /\
-   Fwd.Forw.self{1} = MI.func{1} ++ [1] /\
-   Fwd.Forw.adv{1} = MI.adv{1} /\
-   KeyEx.KEIdeal.self{1} = MI.func{1} ++ [2] /\
-   KeyEx.KEIdeal.adv{1} = MI.adv{1} /\
-   SMCIdeal.self{2} = MI.func{1} /\ SMCIdeal.adv{2} = MI.adv{1} /\
-   SMCSim.self{2} = MI.adv{1} /\ SMCSim.adv{2} = [] /\
-   ={glob Adv} /\
-   (exists (pt1 pt2 : port, x : bits, q : exp),
-    smc_sec2_rel2
-    {|smc_sec2_st_func = MI.func{1}; smc_sec2_st_smcrs = SMCReal.st{1};
-      smc_sec2_st_fws = Fwd.Forw.st{1}; smc_sec2_st_keis = KeyEx.KEIdeal.st{1};
-      smc_sec2_st_smcis = SMCIdeal.st{2}; smc_sec2_st_smcss = SMCSim.st{2}|}
-    pt1 pt2 x q) ==>
-   ={res, MI.func, MI.adv, MI.in_guard} /\
-   exper_pre MI.func{1} MI.adv{1} (fset1 adv_fw_pi) /\
-   MI.in_guard{1} = fset1 adv_fw_pi /\
-   SMCReal.self{1} = MI.func{1} /\ SMCReal.adv{1} = MI.adv{1} /\
-   Fwd.Forw.self{1} = MI.func{1} ++ [1] /\
-   Fwd.Forw.adv{1} = MI.adv{1} /\
-   KeyEx.KEIdeal.self{1} = MI.func{1} ++ [2] /\
-   KeyEx.KEIdeal.adv{1} = MI.adv{1} /\
-   SMCIdeal.self{2} = MI.func{1} /\ SMCIdeal.adv{2} = MI.adv{1} /\
-   SMCSim.self{2} = MI.adv{1} /\ SMCSim.adv{2} = [] /\
-   ={glob Adv} /\
-   smc_sec2_rel_2_4
-   {|smc_sec2_st_func = MI.func{1}; smc_sec2_st_smcrs = SMCReal.st{1};
-     smc_sec2_st_fws = Fwd.Forw.st{1}; smc_sec2_st_keis = KeyEx.KEIdeal.st{1};
-     smc_sec2_st_smcis = SMCIdeal.st{2}; smc_sec2_st_smcss = SMCSim.st{2}|}].
-proof.
-admit.
-qed.
-
-lemma MI_SMCReal_KEIdeal_Adv_SMCIdeal_SMCSim_Adv_invoke_1 :
-  equiv
-  [MI(SMCReal(KeyEx.KEIdeal), Adv).invoke ~
-   MI(SMCIdeal, SMCSim(Adv)).invoke :
-   ={m, MI.func, MI.adv, MI.in_guard} /\
-   exper_pre MI.func{1} MI.adv{1} (fset1 adv_fw_pi) /\
-   MI.in_guard{1} = fset1 adv_fw_pi /\
-   SMCReal.self{1} = MI.func{1} /\ SMCReal.adv{1} = MI.adv{1} /\
-   Fwd.Forw.self{1} = MI.func{1} ++ [1] /\
-   Fwd.Forw.adv{1} = MI.adv{1} /\
-   KeyEx.KEIdeal.self{1} = MI.func{1} ++ [2] /\
-   KeyEx.KEIdeal.adv{1} = MI.adv{1} /\
-   SMCIdeal.self{2} = MI.func{1} /\ SMCIdeal.adv{2} = MI.adv{1} /\
-   SMCSim.self{2} = MI.adv{1} /\ SMCSim.adv{2} = [] /\
-   ={glob Adv} /\
-   (exists (pt1 pt2 : port, x : bits, q : exp),
-    smc_sec2_rel1
-    {|smc_sec2_st_func = MI.func{1}; smc_sec2_st_smcrs = SMCReal.st{1};
-      smc_sec2_st_fws = Fwd.Forw.st{1}; smc_sec2_st_keis = KeyEx.KEIdeal.st{1};
-      smc_sec2_st_smcis = SMCIdeal.st{2}; smc_sec2_st_smcss = SMCSim.st{2}|}
-    pt1 pt2 x q) ==>
-   ={res, MI.func, MI.adv, MI.in_guard} /\
-   exper_pre MI.func{1} MI.adv{1} (fset1 adv_fw_pi) /\
-   MI.in_guard{1} = fset1 adv_fw_pi /\
-   SMCReal.self{1} = MI.func{1} /\ SMCReal.adv{1} = MI.adv{1} /\
-   Fwd.Forw.self{1} = MI.func{1} ++ [1] /\
-   Fwd.Forw.adv{1} = MI.adv{1} /\
-   KeyEx.KEIdeal.self{1} = MI.func{1} ++ [2] /\
-   KeyEx.KEIdeal.adv{1} = MI.adv{1} /\
-   SMCIdeal.self{2} = MI.func{1} /\ SMCIdeal.adv{2} = MI.adv{1} /\
-   SMCSim.self{2} = MI.adv{1} /\ SMCSim.adv{2} = [] /\
-   ={glob Adv} /\
-   smc_sec2_rel_1_4
-   {|smc_sec2_st_func = MI.func{1}; smc_sec2_st_smcrs = SMCReal.st{1};
-     smc_sec2_st_fws = Fwd.Forw.st{1}; smc_sec2_st_keis = KeyEx.KEIdeal.st{1};
-     smc_sec2_st_smcis = SMCIdeal.st{2}; smc_sec2_st_smcss = SMCSim.st{2}|}].
-proof.
-admit.
-qed.
-
-lemma MI_SMCReal_KEIdeal_Adv_SMCIdeal_SMCSim_Adv_invoke_0 :
-  equiv
-  [MI(SMCReal(KeyEx.KEIdeal), Adv).invoke ~
-   MI(SMCIdeal, SMCSim(Adv)).invoke :
-   ={m, MI.func, MI.adv, MI.in_guard} /\
-   exper_pre MI.func{1} MI.adv{1} (fset1 adv_fw_pi) /\
-   MI.in_guard{1} = fset1 adv_fw_pi /\
-   SMCReal.self{1} = MI.func{1} /\ SMCReal.adv{1} = MI.adv{1} /\
-   Fwd.Forw.self{1} = MI.func{1} ++ [1] /\
-   Fwd.Forw.adv{1} = MI.adv{1} /\
-   KeyEx.KEIdeal.self{1} = MI.func{1} ++ [2] /\
-   KeyEx.KEIdeal.adv{1} = MI.adv{1} /\
-   SMCIdeal.self{2} = MI.func{1} /\ SMCIdeal.adv{2} = MI.adv{1} /\
-   SMCSim.self{2} = MI.adv{1} /\ SMCSim.adv{2} = [] /\
-   ={glob Adv} /\
-   smc_sec2_rel0
-   {|smc_sec2_st_func = MI.func{1}; smc_sec2_st_smcrs = SMCReal.st{1};
-     smc_sec2_st_fws = Fwd.Forw.st{1}; smc_sec2_st_keis = KeyEx.KEIdeal.st{1};
-     smc_sec2_st_smcis = SMCIdeal.st{2}; smc_sec2_st_smcss = SMCSim.st{2}|} ==>
-   ={res, MI.func, MI.adv, MI.in_guard} /\
-   exper_pre MI.func{1} MI.adv{1} (fset1 adv_fw_pi) /\
-   MI.in_guard{1} = fset1 adv_fw_pi /\
-   SMCReal.self{1} = MI.func{1} /\ SMCReal.adv{1} = MI.adv{1} /\
-   Fwd.Forw.self{1} = MI.func{1} ++ [1] /\
-   Fwd.Forw.adv{1} = MI.adv{1} /\
-   KeyEx.KEIdeal.self{1} = MI.func{1} ++ [2] /\
-   KeyEx.KEIdeal.adv{1} = MI.adv{1} /\
-   SMCIdeal.self{2} = MI.func{1} /\ SMCIdeal.adv{2} = MI.adv{1} /\
-   SMCSim.self{2} = MI.adv{1} /\ SMCSim.adv{2} = [] /\
-   ={glob Adv} /\
-   smc_sec2_rel
-   {|smc_sec2_st_func = MI.func{1}; smc_sec2_st_smcrs = SMCReal.st{1};
-     smc_sec2_st_fws = Fwd.Forw.st{1}; smc_sec2_st_keis = KeyEx.KEIdeal.st{1};
-     smc_sec2_st_smcis = SMCIdeal.st{2}; smc_sec2_st_smcss = SMCSim.st{2}|}].
-proof.
-proc.
-sp 2 2.
-if => //; last first.
-auto; progress; by apply SMCSec2Rel0.
-inline MI(SMCReal(KeyEx.KEIdeal), Adv).loop
-       MI(SMCIdeal, SMCSim(Adv)).loop.
-sp 3 3.
-rcondt{1} 1; first progress. rcondt{2} 1; first progress.
-sp 2 2.
-if => //.
-inline{1} (1) SMCReal(KeyEx.KEIdeal).invoke.
-inline{2} (1) SMCIdeal.invoke.
-sp 4 4.
-if => //.
-progress; smt(inc_ext2).
-admit.
-rcondt{1} 2; first auto.
-rcondt{2} 2; first auto.
-rcondf{1} 3; first auto.
-rcondf{2} 3; first auto.
-auto; progress; by apply SMCSec2Rel0.
-inline{2} (1) SMCSim(Adv).invoke.
-sp 0 3.
-rcondt{2} 1.
-progress; auto; progress; smt().
-inline{2} (1) SMCSim(Adv).loop.
-rcondt{2} 4; progress; auto.
-sp 0 4.
-rcondf{2} 1; progress; auto; progress.
-have smc_pi_uniq := smc_pi_uniq.
-rewrite cons_uniq 3!in_cons in_nil 2!negb_or /= in smc_pi_uniq.
-smt(in_fset1).
-seq 1 1 :
-   (r0{1} = r2{2} /\ not_done{1} /\ not_done{2} /\
-   ={MI.func, MI.adv, MI.in_guard} /\
-   exper_pre MI.func{1} MI.adv{1} (fset1 adv_fw_pi) /\
-   MI.in_guard{1} = fset1 adv_fw_pi /\
-   SMCReal.self{1} = MI.func{1} /\ SMCReal.adv{1} = MI.adv{1} /\
-   Fwd.Forw.self{1} = MI.func{1} ++ [1] /\
-   Fwd.Forw.adv{1} = MI.adv{1} /\
-   KeyEx.KEIdeal.self{1} = MI.func{1} ++ [2] /\
-   KeyEx.KEIdeal.adv{1} = MI.adv{1} /\
-   SMCIdeal.self{2} = MI.func{1} /\  SMCIdeal.adv{2} = MI.adv{1} /\
-   SMCSim.self{2} = MI.adv{1} /\ SMCSim.adv{2} = [] /\
-   ={glob Adv} /\
-   smc_sec2_rel0
-   {|smc_sec2_st_func = MI.func{1}; smc_sec2_st_smcrs = SMCReal.st{1};
-     smc_sec2_st_fws = Fwd.Forw.st{1}; smc_sec2_st_keis = KeyEx.KEIdeal.st{1};
-     smc_sec2_st_smcis = SMCIdeal.st{2}; smc_sec2_st_smcss = SMCSim.st{2};|}).
-call (_ : true).
-auto.
-if => //.
-rcondf{1} 2; first auto.
-rcondf{2} 2; first auto.
-rcondt{2} 4; first auto.
-rcondf{2} 5; first auto.
-auto; progress; by apply SMCSec2Rel0.
-sp 3 2.
-rcondf{2} 1; first auto; progress; smt().
-rcondf{2} 1; first auto; progress; smt().
-rcondf{2} 1; first auto; progress; smt().
-rcondf{2} 2; first auto.
-rcondf{2} 4; first auto.
-sp 0 6.
-if => //.
-move => |> &1 &2 <- //.
-rcondf{1} 3; first auto.
-rcondf{2} 3; first auto.
-auto; progress; by apply SMCSec2Rel0.
-if => //.
-move => |> &1 &2 <- //.
-rcondf{1} 2; first auto.
-rcondf{2} 2; first auto.
-auto; progress; by apply SMCSec2Rel0.
-rcondt{1} 1; first auto. rcondt{2} 1; first auto.
-sp 2 2.
-elim* => addr10_R n10_R mod0_R pt10_R pt20_R u0_R addr10_L n10_L mod0_L
-         pt10_L pt20_L u0_L.
-rcondt{1} 1; first auto.
-rcondt{2} 1; first progress; auto => |> &hr <- //.
-inline{1} (1) SMCReal(KeyEx.KEIdeal).invoke.
-inline{2} (1) SMCIdeal.invoke.
-sp 4 4.
-conseq
-  (_ :
-   _ ==>
-   r0{1} = None /\ r0{2} = None /\
-   ={MI.func, MI.adv, MI.in_guard} /\
-   exper_pre MI.func{1} MI.adv{1} (fset1 adv_fw_pi) /\
-   MI.in_guard{1} = fset1 adv_fw_pi /\
-   SMCReal.self{1} = MI.func{1} /\
-   SMCReal.adv{1} = MI.adv{1} /\
-   Fwd.Forw.self{1} = MI.func{1} ++ [1] /\
-   Fwd.Forw.adv{1} = MI.adv{1} /\
-   KeyEx.KEIdeal.self{1} = MI.func{1} ++ [2] /\
-   KeyEx.KEIdeal.adv{1} = MI.adv{1} /\
-   SMCIdeal.self{2} = MI.func{1} /\
-   SMCIdeal.adv{2} = MI.adv{1} /\
-   SMCSim.self{2} = MI.adv{1} /\
-   SMCSim.adv{2} = [] /\
-   ={glob Adv} /\
-   smc_sec2_rel
-    {|smc_sec2_st_func = MI.func{1}; smc_sec2_st_smcrs = SMCReal.st{1};
-      smc_sec2_st_fws = Fwd.Forw.st{1}; smc_sec2_st_keis = KeyEx.KEIdeal.st{1};
-      smc_sec2_st_smcis = SMCIdeal.st{2}; smc_sec2_st_smcss = SMCSim.st{2};|}) => //.
-rcondf{2} 1.
-auto => |> &hr <-; progress; smt().
-rcondt{2} 2; first auto.
-rcondf{2} 3; first auto.
-if{1}.
-inline{1} (1) SMCReal(KeyEx.KEIdeal).loop.
-rcondt{1} 4; first auto.
-sp 3 0.
-if{1}.
-inline{1} (1) SMCReal(KeyEx.KEIdeal).parties.
-sp 2 0.
-rcondt{1} 1.
-progress; auto; progress; smt().
-rcondf{1} 1.
-progress; auto; progress.
-rewrite /is_smc_req /dec_smc_req /#.
-rcondt{1} 2; first auto.
-rcondf{1} 3; first auto.
-rcondt{1} 5.
-progress; auto; progress.
-rcondf{1} 6; first auto.
-auto; progress; by apply SMCSec2Rel0.
-if{1}.
-inline{1} (1) Fwd.Forw.invoke.
-rcondt{1} 3.
-progress; auto; smt().
-rcondf{1} 3.
-progress; auto; progress.
-rewrite /is_fw_req /dec_fw_req /#.
-rcondt{1} 4; first auto.
-rcondf{1} 5; first auto.
-rcondt{1} 7; first auto.
-rcondf{1} 8; first auto.
-auto; progress; by apply SMCSec2Rel0.
-inline{1} (1) KeyEx.KEIdeal.invoke.
-rcondf{1} 5.
-progress; auto; progress; smt().
-rcondf{1} 6; first auto.
-rcondt{1} 6; first auto.
-rcondf{1} 7; first auto.
-rcondt{1} 9; first auto.
-rcondf{1} 10; first auto.
-auto; progress; by apply SMCSec2Rel0.
-rcondt{1} 2; first auto.
-rcondf{1} 3; first auto.
-auto; progress; by apply SMCSec2Rel0.
-qed.
-
-lemma MI_SMCReal_KEIdeal_Adv_SMCIdeal_SMCSim_Adv_invoke :
-  equiv
-  [MI(SMCReal(KeyEx.KEIdeal), Adv).invoke ~
-   MI(SMCIdeal, SMCSim(Adv)).invoke :
-   ={m, MI.func, MI.adv, MI.in_guard} /\
-   exper_pre MI.func{1} MI.adv{1} (fset1 adv_fw_pi) /\
-   MI.in_guard{1} = fset1 adv_fw_pi /\
-   SMCReal.self{1} = MI.func{1} /\ SMCReal.adv{1} = MI.adv{1} /\
-   Fwd.Forw.self{1} = MI.func{1} ++ [1] /\
-   Fwd.Forw.adv{1} = MI.adv{1} /\
-   KeyEx.KEIdeal.self{1} = MI.func{1} ++ [2] /\
-   KeyEx.KEIdeal.adv{1} = MI.adv{1} /\
-   SMCIdeal.self{2} = MI.func{1} /\ SMCIdeal.adv{2} = MI.adv{1} /\
-   SMCSim.self{2} = MI.adv{1} /\ SMCSim.adv{2} = [] /\
-   ={glob Adv} /\
-   smc_sec2_rel
-   {|smc_sec2_st_func = MI.func{1}; smc_sec2_st_smcrs = SMCReal.st{1};
-     smc_sec2_st_fws = Fwd.Forw.st{1}; smc_sec2_st_keis = KeyEx.KEIdeal.st{1};
-     smc_sec2_st_smcis = SMCIdeal.st{2}; smc_sec2_st_smcss = SMCSim.st{2}|} ==>
-   ={res, MI.func, MI.adv, MI.in_guard} /\
-   exper_pre MI.func{1} MI.adv{1} (fset1 adv_fw_pi) /\
-   MI.in_guard{1} = fset1 adv_fw_pi /\
-   SMCReal.self{1} = MI.func{1} /\ SMCReal.adv{1} = MI.adv{1} /\
-   Fwd.Forw.self{1} = MI.func{1} ++ [1] /\
-   Fwd.Forw.adv{1} = MI.adv{1} /\
-   KeyEx.KEIdeal.self{1} = MI.func{1} ++ [2] /\
-   KeyEx.KEIdeal.adv{1} = MI.adv{1} /\
-   SMCIdeal.self{2} = MI.func{1} /\ SMCIdeal.adv{2} = MI.adv{1} /\
-   SMCSim.self{2} = MI.adv{1} /\ SMCSim.adv{2} = [] /\
-   ={glob Adv} /\
-   smc_sec2_rel
-   {|smc_sec2_st_func = MI.func{1}; smc_sec2_st_smcrs = SMCReal.st{1};
-     smc_sec2_st_fws = Fwd.Forw.st{1}; smc_sec2_st_keis = KeyEx.KEIdeal.st{1};
-     smc_sec2_st_smcis = SMCIdeal.st{2}; smc_sec2_st_smcss = SMCSim.st{2}|}].
-proof.
-proc*.
-case
-  (smc_sec2_rel0
-   {|smc_sec2_st_func = MI.func{1}; smc_sec2_st_smcrs = SMCReal.st{1};
-     smc_sec2_st_fws = Fwd.Forw.st{1}; smc_sec2_st_keis = KeyEx.KEIdeal.st{1};
-     smc_sec2_st_smcis = SMCIdeal.st{2}; smc_sec2_st_smcss = SMCSim.st{2};|}).
-call MI_SMCReal_KEIdeal_Adv_SMCIdeal_SMCSim_Adv_invoke_0.
-auto.
-case
-  (exists (pt1 pt2 : port, x : bits, q : exp),
-   smc_sec2_rel1
-   {|smc_sec2_st_func = MI.func{1}; smc_sec2_st_smcrs = SMCReal.st{1};
-     smc_sec2_st_fws = Fwd.Forw.st{1}; smc_sec2_st_keis = KeyEx.KEIdeal.st{1};
-     smc_sec2_st_smcis = SMCIdeal.st{2}; smc_sec2_st_smcss = SMCSim.st{2};|}
-   pt1 pt2 x q).
-call MI_SMCReal_KEIdeal_Adv_SMCIdeal_SMCSim_Adv_invoke_1.
-auto; progress.
-by exists pt1 pt2 x q.
-by apply smc_sec2_rel_1_4_imp_full.
-case
-  (exists (pt1 pt2 : port, x : bits, q : exp),
-   smc_sec2_rel2
-   {|smc_sec2_st_func = MI.func{1}; smc_sec2_st_smcrs = SMCReal.st{1};
-     smc_sec2_st_fws = Fwd.Forw.st{1}; smc_sec2_st_keis = KeyEx.KEIdeal.st{1};
-     smc_sec2_st_smcis = SMCIdeal.st{2}; smc_sec2_st_smcss = SMCSim.st{2};|}
-   pt1 pt2 x q).
-call MI_SMCReal_KEIdeal_Adv_SMCIdeal_SMCSim_Adv_invoke_2.
-auto; progress.
-by exists pt1 pt2 x q.
-by apply smc_sec2_rel_2_4_imp_full.
-case
-  (exists (pt1 pt2 : port, x : bits, q : exp),
-   smc_sec2_rel3
-   {|smc_sec2_st_func = MI.func{1}; smc_sec2_st_smcrs = SMCReal.st{1};
-     smc_sec2_st_fws = Fwd.Forw.st{1}; smc_sec2_st_keis = KeyEx.KEIdeal.st{1};
-     smc_sec2_st_smcis = SMCIdeal.st{2}; smc_sec2_st_smcss = SMCSim.st{2};|}
-   pt1 pt2 x q).
-call MI_SMCReal_KEIdeal_Adv_SMCIdeal_SMCSim_Adv_invoke_3.
-auto; progress.
-by exists pt1 pt2 x q.
-by apply smc_sec2_rel_3_4_imp_full.
-case
-  (exists (pt1 pt2 : port, x : bits, q : exp),
-   smc_sec2_rel4
-   {|smc_sec2_st_func = MI.func{1}; smc_sec2_st_smcrs = SMCReal.st{1};
-     smc_sec2_st_fws = Fwd.Forw.st{1}; smc_sec2_st_keis = KeyEx.KEIdeal.st{1};
-     smc_sec2_st_smcis = SMCIdeal.st{2}; smc_sec2_st_smcss = SMCSim.st{2};|}
-   pt1 pt2 x q).
-call MI_SMCReal_KEIdeal_Adv_SMCIdeal_SMCSim_Adv_invoke_4.
-auto; progress.
-by exists pt1 pt2 x q.
-by apply smc_sec2_rel_4_imp_full.
-exfalso => &1 &2 [# _ _ _ _ _ _ _ _ _ _ _ _ _ _ _ _ _].
-case => //.
-move => pt1 pt2 x q true1 _ false1.
-have true1_ex // : 
-  exists (pt1 pt2 : port, x : bits, q : exp),
-  smc_sec2_rel1
-   {|smc_sec2_st_func = MI.func{1}; smc_sec2_st_smcrs = SMCReal.st{1};
-     smc_sec2_st_fws = Fwd.Forw.st{1}; smc_sec2_st_keis = KeyEx.KEIdeal.st{1};
-     smc_sec2_st_smcis = SMCIdeal.st{2}; smc_sec2_st_smcss = SMCSim.st{2};|}
-  pt1 pt2 x q.
-  by exists pt1 pt2 x q.
-move => pt1 pt2 x q true2 _ _.
-have true2_ex // : 
-  exists (pt1 pt2 : port, x : bits, q : exp),
-  smc_sec2_rel2
-   {|smc_sec2_st_func = MI.func{1}; smc_sec2_st_smcrs = SMCReal.st{1};
-     smc_sec2_st_fws = Fwd.Forw.st{1}; smc_sec2_st_keis = KeyEx.KEIdeal.st{1};
-     smc_sec2_st_smcis = SMCIdeal.st{2}; smc_sec2_st_smcss = SMCSim.st{2};|}
-  pt1 pt2 x q.
-  by exists pt1 pt2 x q.
-move => pt1 pt2 x q true3 _ _ _.
-have true3_ex // : 
-  exists (pt1 pt2 : port, x : bits, q : exp),
-  smc_sec2_rel3
-   {|smc_sec2_st_func = MI.func{1}; smc_sec2_st_smcrs = SMCReal.st{1};
-     smc_sec2_st_fws = Fwd.Forw.st{1}; smc_sec2_st_keis = KeyEx.KEIdeal.st{1};
-     smc_sec2_st_smcis = SMCIdeal.st{2}; smc_sec2_st_smcss = SMCSim.st{2};|}
-  pt1 pt2 x q.
-  by exists pt1 pt2 x q.
-move => pt1 pt2 x q true4 _ _ _.
-have true4_ex // : 
-  exists (pt1 pt2 : port, x : bits, q : exp),
-  smc_sec2_rel4
-   {|smc_sec2_st_func = MI.func{1}; smc_sec2_st_smcrs = SMCReal.st{1};
-     smc_sec2_st_fws = Fwd.Forw.st{1}; smc_sec2_st_keis = KeyEx.KEIdeal.st{1};
-     smc_sec2_st_smcis = SMCIdeal.st{2}; smc_sec2_st_smcss = SMCSim.st{2};|}
-  pt1 pt2 x q.
-  by exists pt1 pt2 x q.
-qed.
+local clone import SMCRealKEIdealSimp as SRKEIS.
 
 lemma smc_sec2 (func adv : addr) &m :
   exper_pre func adv (fset1 adv_fw_pi) =>
@@ -1621,71 +1256,18 @@ lemma smc_sec2 (func adv : addr) &m :
   Pr[Exper(MI(SMCIdeal, SMCSim(Adv)), Env).main
        (func, adv, fset1 adv_fw_pi) @ &m : res].
 proof.
-move => pre; byequiv => //; proc.
-seq 1 1 :
-  (={func, adv, in_guard, MI.func, MI.adv, MI.in_guard} /\
-   exper_pre func{1} adv{1} (fset1 adv_fw_pi) /\
-   MI.func{1} = func{1} /\ MI.adv{1} = adv{1} /\
-   MI.in_guard{1} = fset1 adv_fw_pi /\
-   SMCReal.self{1} = func{1} /\ SMCReal.adv{1} = adv{1} /\
-   SMCReal.st{1} = SMCRealStateWaitReq /\
-   Fwd.Forw.self{1} = func{1} ++ [1] /\ Fwd.Forw.adv{1} = adv{1} /\
-   Fwd.Forw.st{1} = Fwd.FwStateInit /\
-   KeyEx.KEIdeal.self{1} = func{1} ++ [2] /\ KeyEx.KEIdeal.adv{1} = adv{1} /\
-   KeyEx.KEIdeal.st{1} = KeyEx.KEIdealStateWaitReq1 /\
-   SMCIdeal.self{2} = func{1} /\ SMCIdeal.adv{2} = adv{1} /\
-   SMCIdeal.st{2} = SMCIdealStateWaitReq /\
-   SMCSim.self{2} = adv{1} /\ SMCSim.adv{2} = [] /\
-   SMCSim.st{2} = SMCSimStateWaitReq /\
-   ={glob Adv}).
-inline*.
-swap{2} 16 1; call (_ : true).
-auto.
-auto.
-call
-  (_ : 
-   ={func, adv, in_guard, MI.func, MI.adv, MI.in_guard} /\
-   exper_pre func{1} adv{1} (fset1 adv_fw_pi) /\
-   MI.func{1} = func{1} /\ MI.adv{1} = adv{1} /\
-   MI.in_guard{1} = fset1 adv_fw_pi /\
-   SMCReal.self{1} = func{1} /\ SMCReal.adv{1} = adv{1} /\
-   Fwd.Forw.self{1} = func{1} ++ [1] /\ Fwd.Forw.adv{1} = adv{1} /\
-   KeyEx.KEIdeal.self{1} = func{1} ++ [2] /\ KeyEx.KEIdeal.adv{1} = adv{1} /\
-   SMCIdeal.self{2} = func{1} /\ SMCIdeal.adv{2} = adv{1} /\
-   SMCSim.self{2} = adv{1} /\ SMCSim.adv{2} = [] /\
-   ={glob Adv} /\
-   smc_sec2_rel
-   {|smc_sec2_st_func = func{1}; smc_sec2_st_smcrs = SMCReal.st{1};
-     smc_sec2_st_fws = Fwd.Forw.st{1}; smc_sec2_st_keis = KeyEx.KEIdeal.st{1};
-     smc_sec2_st_smcis = SMCIdeal.st{2}; smc_sec2_st_smcss = SMCSim.st{2}|} ==>
-   ={res}).
-proc
-  (={MI.func, MI.adv, MI.in_guard} /\
-   exper_pre func{1} adv{1} (fset1 adv_fw_pi) /\
-   MI.func{1} = func{1} /\ MI.adv{1} = adv{1} /\
-   MI.in_guard{1} = fset1 adv_fw_pi /\
-   SMCReal.self{1} = func{1} /\ SMCReal.adv{1} = adv{1} /\
-   Fwd.Forw.self{1} = func{1} ++ [1] /\ Fwd.Forw.adv{1} = adv{1} /\
-   KeyEx.KEIdeal.self{1} = func{1} ++ [2] /\ KeyEx.KEIdeal.adv{1} = adv{1} /\
-   SMCIdeal.self{2} = func{1} /\ SMCIdeal.adv{2} = adv{1} /\
-   SMCSim.self{2} = adv{1} /\ SMCSim.adv{2} = [] /\
-   ={glob Adv} /\
-   smc_sec2_rel
-   {|smc_sec2_st_func = func{1}; smc_sec2_st_smcrs = SMCReal.st{1};
-     smc_sec2_st_fws = Fwd.Forw.st{1}; smc_sec2_st_keis = KeyEx.KEIdeal.st{1};
-     smc_sec2_st_smcis = SMCIdeal.st{2}; smc_sec2_st_smcss = SMCSim.st{2}|}) => //.
-by conseq MI_SMCReal_KEIdeal_Adv_SMCIdeal_SMCSim_Adv_invoke.
-auto; progress; by apply SMCSec2Rel0.
+move => pre.
+rewrite (Exper_SMCReal_KEIdeal_SMCRealKEIdealSimp func adv (fset1 adv_fw_pi)
+         &m Adv Env) 1:/#.
+admit.
 qed.
 
 end section.
-*)
-
 
 lemma smc_security2
-        (Adv <: FUNC{MI, SMCReal, SMCIdeal, SMCSim, KeyEx.KEIdeal})
-        (Env <: ENV{Adv, MI, SMCReal, SMCIdeal, SMCSim, KeyEx.KEIdeal})
-        (func adv : addr) &m :
+      (Adv <: FUNC{MI, SMCReal, SMCIdeal, SMCSim, KeyEx.KEIdeal})
+      (Env <: ENV{Adv, MI, SMCReal, SMCIdeal, SMCSim, KeyEx.KEIdeal})
+      (func adv : addr) &m :
   exper_pre func adv (fset1 adv_fw_pi) =>
   Pr[Exper(MI(SMCReal(KeyEx.KEIdeal), Adv), Env).main
        (func, adv, fset1 adv_fw_pi) @ &m : res] =
@@ -1693,18 +1275,15 @@ lemma smc_security2
        (func, adv, fset1 adv_fw_pi) @ &m : res].
 proof.
 move => pre.
-(*
 by apply (smc_sec2 Adv Env func adv &m).
-*)
-admit.
 qed.
 
 lemma smc_security
-        (Adv <: FUNC{MI, SMCReal, SMCIdeal, SMCSim, KeyEx.KEReal,
-                     KeyEx.KEIdeal, KeyEx.KESim, KeyEx.DDH_Adv, CompEnv})
-        (Env <: ENV{Adv, MI, SMCReal, SMCIdeal, SMCSim, KeyEx.KEReal,
-                    KeyEx.KEIdeal, KeyEx.KESim, KeyEx.DDH_Adv, CompEnv})
-        (func adv : addr) &m :
+      (Adv <: FUNC{MI, SMCReal, SMCIdeal, SMCSim, KeyEx.KEReal,
+                   KeyEx.KEIdeal, KeyEx.KESim, KeyEx.DDH_Adv, CompEnv})
+      (Env <: ENV{Adv, MI, SMCReal, SMCIdeal, SMCSim, KeyEx.KEReal,
+                  KeyEx.KEIdeal, KeyEx.KESim, KeyEx.DDH_Adv, CompEnv})
+      (func adv : addr) &m :
   exper_pre func adv (fset1 adv_fw_pi) =>
   KeyEx.DDH_Adv.func{m} = func ++ [2] => KeyEx.DDH_Adv.adv{m} = adv =>
   `|Pr[Exper(MI(SMCReal(KeyEx.KEReal), Adv), Env).main
